code/experimental/rsapss/Hacl.Spec.Bignum.Montgomery.fsti
@@ -20,10 +20,15 @@ val mod_inv_u64_lemma: n0:uint64 -> Lemma
   (requires v n0 % 2 == 1)
   (ensures (1 + v n0 * v (mod_inv_u64 n0)) % pow2 64 == 0)
 
-///
-///  TODO: compute constant R2 == R * R % N, where R = pow2 (64 * rLen)
-///
+val precomp_r2_mod_n: #nLen:size_nat -> n:lbignum nLen -> lbignum nLen
 
+val precomp_r2_mod_n_lemma: #nLen:size_nat -> n:lbignum nLen -> Lemma
+  (requires bn_v n > 0)
+  (ensures  bn_v (precomp_r2_mod_n n) == pow2 (128 * (nLen + 1)) % bn_v n)
+
+///
+///  Conversion functions to/from the Montgomery domen and the Montgomery reduction
+///
 
 val mont_reduction:
     #nLen:size_nat
