code/experimental/rsapss/Hacl.Spec.Bignum.fsti
@@ -75,6 +75,11 @@ val bn_is_bit_set: #len:size_nat -> b:lbignum len -> i:size_nat{i / 64 < len} ->
 val bn_is_bit_set_lemma: #len:size_nat -> b:lbignum len -> i:size_nat{i / 64 < len} ->
   Lemma (bn_is_bit_set b i == (bn_v b / pow2 i % 2 = 1))
 
+val bn_bit_set: #len:size_nat -> b:lbignum len -> i:size_nat{i / 64 < len} -> lbignum len
+
+val bn_bit_set_lemma: #len:size_nat -> b:lbignum len -> i:size_nat{i / 64 < len} -> Lemma
+  (requires bn_v b < pow2 i)
+  (ensures  bn_v (bn_bit_set b i) == bn_v b + pow2 i)
 
 ///
 ///  Conversion functions for bignum
